exercises/chapter03-state-machines/exercise02.dfy
@@ -13,17 +13,20 @@
 
 // Define all the relevant state in this datatype.
 // FIXME: fill in here (solution: 8 lines)
- datatype Variables = Variables(tableSize: nat)
- {
-   ghost predicate WellFormed() {
-     && 0 < tableSize
-   }
- }
+datatype ChopstickState = Available | AcquiredAsLeft | AcquiredAsRight
+datatype Variables = Variables(tableSize: nat, chopsticks: seq<ChopstickState>)
+{
+  ghost predicate WellFormed() {
+    && 0 < tableSize
+    && |chopsticks| == tableSize
+  }
+}
 // END EDIT
 
 ghost predicate Init(v:Variables) {
   // FIXME: fill in here (solution: 3 lines)
-      true  // Replace me
+  && v.WellFormed()
+  && forall i | 0 <= i < v.tableSize :: v.chopsticks[i].Available?
   // END EDIT
 }
 
@@ -34,33 +37,45 @@ ghost predicate Init(v:Variables) {
 // Philosopher with index philosopherIndex acquires left chopstick
 ghost predicate AcquireLeft(v:Variables, v':Variables, philosopherIndex:nat) {
   // FIXME: fill in here (solution: 5 lines)
-      true  // Replace me
+  && 0 <= philosopherIndex < |v.chopsticks|
+  && v.chopsticks[philosopherIndex] == Available
+  && v' == v.(chopsticks := v.chopsticks[philosopherIndex := AcquiredAsLeft])
   // END EDIT
 }
 
 // Philosopher with index philosopherIndex acquires right chopstick
 ghost predicate AcquireRight(v:Variables, v':Variables, philosopherIndex:nat) {
   // FIXME: fill in here (solution: 5 lines)
-      true  // Replace me
+  && 0 <= philosopherIndex < |v.chopsticks|
+  && v.chopsticks[(philosopherIndex + 1) % |v.chopsticks|] == Available
+  && v' == v.(chopsticks := v.chopsticks[(philosopherIndex + 1) % |v.chopsticks| := AcquiredAsRight])
   // END EDIT
 }
 
 // Philosopher with index philosopherIndex releases both chopsticks
 ghost predicate ReleaseBoth(v:Variables, v':Variables, philosopherIndex:nat) {
   // FIXME: fill in here (solution: 5 lines)
-      true  // Replace me
+  && 0 <= philosopherIndex < |v.chopsticks|
+  && v.chopsticks[philosopherIndex] == AcquiredAsLeft
+  && v.chopsticks[(philosopherIndex + 1) % |v.chopsticks|] == AcquiredAsRight
+  && v' == v.(chopsticks := v.chopsticks[philosopherIndex := Available])
+  && v' == v.(chopsticks := v.chopsticks[(philosopherIndex + 1) % |v.chopsticks| := Available])
   // END EDIT
 }
 
 datatype Step =
     // FIXME: fill in here (solution: 3 lines)
-     Step()  // Replace me
+    | AcquireLeft(philosopherIndex:nat)
+    | AcquireRight(philosopherIndex:nat)
+    | ReleaseBoth(philosopherIndex:nat)
     // END EDIT
 
 ghost predicate NextStep(v:Variables, v':Variables, step: Step) {
   match step
   // FIXME: fill in here (solution: 3 lines)
-   case Step => false  // Replace me
+  case AcquireLeft(philosopherIndex) => AcquireLeft(v, v', philosopherIndex)
+  case AcquireRight(philosopherIndex) => AcquireRight(v, v', philosopherIndex)
+  case ReleaseBoth(philosopherIndex) => ReleaseBoth(v, v', philosopherIndex)
   // END EDIT
 }
 
@@ -81,7 +96,7 @@ ghost predicate NoSticksAcquired(v: Variables)
   requires v.WellFormed()
 {
   // FIXME: fill in here (solution: 8 lines)
-          true // Replace me
+  forall i | 0 <= i < |v.chopsticks| :: v.chopsticks[i].Available?
   // END EDIT
 }
 
@@ -94,7 +109,8 @@ ghost predicate BothSticksAcquired(v: Variables, philosopherIndex: nat)
   requires v.WellFormed()
 {
   // FIXME: fill in here (solution: 6 lines)
-      true
+  && v.chopsticks[philosopherIndex] == AcquiredAsLeft
+  && v.chopsticks[(philosopherIndex + 1) % |v.chopsticks|] == AcquiredAsRight
   // END EDIT
 }
 
@@ -121,5 +137,12 @@ lemma PseudoLiveness(philosopherIndex:nat) returns (behavior:seq<Variables>)
   ensures BothSticksAcquired(behavior[|behavior|-1], philosopherIndex)  // Behavior ultimately achieves acquisition for philosopherIndex
 {
   // FIXME: fill in here (solution: 6 lines)
+  var v1 := Variables(tableSize := 3, chopsticks := [Available, Available, Available]);
+  assert Init(v1);
+  var v2 := v1.(chopsticks := [Available, AcquiredAsLeft, Available]);
+  assert NextStep(v1, v2, Step.AcquireLeft(philosopherIndex));
+  var v3 := v1.(chopsticks := [Available, AcquiredAsLeft, AcquiredAsRight]);
+  assert NextStep(v2, v3, Step.AcquireRight(philosopherIndex));
+  behavior := [v1, v2, v3];
   // END EDIT
 }
